Prove wp_createPersistentVolumeClaims

src/proof/controllers/statefulset/create_pvc.v
@@ -1,6 +1,7 @@
 From New.proof Require Import prelude empty_ffi.
 From New.proof.controllers.statefulset Require Export pvc.
-From New.proof.kubernetes_model Require Export create_named_orphan.
+From New.proof.kubernetes_model Require Export create_named_orphan get_reserved.
+From New.proof.map Require Import for_range.
 
 Section proof.
 Context `{hG: !heapGS Σ} `{!ffi_semantics _ _}.
@@ -48,39 +49,262 @@ Definition new_persistent_volume_claim_key
   PersistentVolumeClaimV.key
     (new_persistent_volume_claim set claim_template ordinal).
 
-(* The controller only needs metadata and spec fragments to remember that the
-   PVC exists.  The model's metadata-fragment validity ties the UID used by
-   both fragments to the PVC metadata. *)
-Definition persistent_volume_claim_exists γ key : iProp Σ :=
-  ∃ claim,
-    "%Hkey" ∷ ⌜ PersistentVolumeClaimV.key claim = key ⌝ ∗
-    "Hmeta" ∷ own_meta_frag γ key
-      claim.(PersistentVolumeClaimV.ObjectMeta').(ObjectMetaV.UID') 1
-      claim.(PersistentVolumeClaimV.ObjectMeta') ∗
-    "Hspec" ∷ own_spec_frag γ key
-      claim.(PersistentVolumeClaimV.ObjectMeta').(ObjectMetaV.UID') 1
-      (ObjectSpecV.PersistentVolumeClaimSpec
-        claim.(PersistentVolumeClaimV.Spec')).
+Lemma new_persistent_volume_claim_key_eq set claim_template ordinal :
+  new_persistent_volume_claim_key set claim_template ordinal =
+    desired_pvc_key set
+      claim_template.(PersistentVolumeClaimV.ObjectMeta').(ObjectMetaV.Name')
+      ordinal.
+Proof.
+  unfold new_persistent_volume_claim_key, PersistentVolumeClaimV.key,
+    PersistentVolumeClaimV.meta_key, desired_pvc_key,
+    new_persistent_volume_claim.
+  done.
+Qed.
+
+Definition persistent_volume_claim_template_insert
+    (claim_templates : gmap go_string PersistentVolumeClaimV.t)
+    (claim_template : PersistentVolumeClaimV.t) :
+    gmap go_string PersistentVolumeClaimV.t :=
+  <[claim_template.(PersistentVolumeClaimV.ObjectMeta').(ObjectMetaV.Name') :=
+    claim_template]> claim_templates.
+
+Definition persistent_volume_claim_templates_by_name
+    (claim_templates : list PersistentVolumeClaimV.t) :
+    gmap go_string PersistentVolumeClaimV.t :=
+  fold_left persistent_volume_claim_template_insert claim_templates ∅.
+
+Lemma persistent_volume_claim_templates_by_name_snoc claim_templates
+    claim_template :
+  persistent_volume_claim_templates_by_name
+      (claim_templates ++ [claim_template]) =
+    persistent_volume_claim_template_insert
+      (persistent_volume_claim_templates_by_name claim_templates)
+      claim_template.
+Proof.
+  unfold persistent_volume_claim_templates_by_name.
+  by rewrite fold_left_app.
+Qed.
+
+Lemma persistent_volume_claim_templates_by_name_dom claim_templates :
+  dom (persistent_volume_claim_templates_by_name claim_templates) =
+    list_to_set
+      ((λ claim_template,
+          claim_template.(PersistentVolumeClaimV.ObjectMeta').(ObjectMetaV.Name'))
+        <$> claim_templates).
+Proof.
+  induction claim_templates using rev_ind.
+  - rewrite /persistent_volume_claim_templates_by_name /=
+      dom_empty_L. done.
+  - apply leibniz_equiv. apply set_equiv.
+    intros name.
+    assert (is_Some
+        (persistent_volume_claim_templates_by_name claim_templates !! name) ↔
+      name ∈ list_to_set (C:=gset go_string)
+        ((λ claim_template,
+            claim_template.(PersistentVolumeClaimV.ObjectMeta').(ObjectMetaV.Name'))
+          <$> claim_templates)) as Hprevious.
+    { rewrite -elem_of_dom IHclaim_templates. done. }
+    rewrite persistent_volume_claim_templates_by_name_snoc
+      /persistent_volume_claim_template_insert.
+    rewrite elem_of_dom lookup_insert_is_Some'.
+    rewrite fmap_app elem_of_list_to_set elem_of_app /=.
+    rewrite Hprevious elem_of_list_to_set.
+    rewrite list_elem_of_singleton.
+    split; intros [Hname|Hprevious'];
+      [right; symmetry; exact Hname
+      |left; exact Hprevious'
+      |right; exact Hname
+      |left; symmetry; exact Hprevious'].
+Qed.
+
+Definition claim_template_maps_related
+    (R : v1.PersistentVolumeClaim.t → PersistentVolumeClaimV.t → Prop)
+    (physical : gmap go_string v1.PersistentVolumeClaim.t)
+    (pure : gmap go_string PersistentVolumeClaimV.t) : Prop :=
+  ∀ name physical_claim_template,
+    physical !! name = Some physical_claim_template →
+    ∃ pure_claim_template,
+      pure !! name = Some pure_claim_template ∧
+      R physical_claim_template pure_claim_template.
+
+Lemma claim_template_maps_related_insert R physical pure
+    physical_claim_template pure_claim_template :
+  physical_claim_template.(v1.PersistentVolumeClaim.ObjectMeta').(v1.ObjectMeta.Name') =
+    pure_claim_template.(PersistentVolumeClaimV.ObjectMeta').(ObjectMetaV.Name') →
+  R physical_claim_template pure_claim_template →
+  claim_template_maps_related R physical pure →
+  claim_template_maps_related R
+    (claim_templates_map_insert physical physical_claim_template)
+    (persistent_volume_claim_template_insert pure pure_claim_template).
+Proof.
+  intros Hname Hindex Hrelated name claim_template Hlookup.
+  unfold claim_templates_map_insert in Hlookup.
+  unfold persistent_volume_claim_template_insert.
+  apply lookup_insert_Some in Hlookup as
+    [[Hkey Hclaim_template]|[Hkey Hlookup]].
+  - subst name claim_template.
+    exists pure_claim_template.
+    rewrite -Hname lookup_insert_eq.
+    split; done.
+  - destruct (Hrelated _ _ Hlookup) as
+      (pure_claim_template' & Hpure & Hindex').
+    exists pure_claim_template'.
+    rewrite lookup_insert_ne.
+    + intros Heq. apply Hkey. rewrite Hname. exact Heq.
+    + split; done.
+Qed.
+
+Lemma Forall2_claim_template_names_with_lookup
+    physical_claim_templates pure_claim_templates :
+  Forall2
+    (λ physical_claim_template pure_claim_template,
+      physical_claim_template.(v1.PersistentVolumeClaim.ObjectMeta').(v1.ObjectMeta.Name') =
+        pure_claim_template.(PersistentVolumeClaimV.ObjectMeta').(ObjectMetaV.Name'))
+    physical_claim_templates pure_claim_templates →
+  Forall2
+    (λ physical_claim_template pure_claim_template,
+      physical_claim_template.(v1.PersistentVolumeClaim.ObjectMeta').(v1.ObjectMeta.Name') =
+        pure_claim_template.(PersistentVolumeClaimV.ObjectMeta').(ObjectMetaV.Name') ∧
+      ∃ i,
+        physical_claim_templates !! i = Some physical_claim_template ∧
+        pure_claim_templates !! i = Some pure_claim_template)
+    physical_claim_templates pure_claim_templates.
+Proof.
+  intros Hclaim_templates.
+  induction Hclaim_templates as
+      [|physical_claim_template pure_claim_template
+         physical_claim_templates pure_claim_templates
+         Hname Hclaim_templates IH];
+    constructor; first split.
+  - exact Hname.
+  - exists 0%nat. done.
+  - eapply Forall2_impl.
+    2: exact IH.
+    intros physical_claim_template' pure_claim_template'
+      (Hname' & i & Hphysical & Hpure).
+    split; first done. exists (S i). simpl. split; done.
+Qed.
+
+Lemma claim_template_maps_related_fold R physical_claim_templates
+    pure_claim_templates physical pure :
+  Forall2
+    (λ physical_claim_template pure_claim_template,
+      physical_claim_template.(v1.PersistentVolumeClaim.ObjectMeta').(v1.ObjectMeta.Name') =
+        pure_claim_template.(PersistentVolumeClaimV.ObjectMeta').(ObjectMetaV.Name') ∧
+      R physical_claim_template pure_claim_template)
+    physical_claim_templates pure_claim_templates →
+  claim_template_maps_related R physical pure →
+  claim_template_maps_related R
+    (fold_left claim_templates_map_insert physical_claim_templates physical)
+    (fold_left persistent_volume_claim_template_insert
+      pure_claim_templates pure).
+Proof.
+  intros Hclaim_templates.
+  revert physical pure.
+  induction Hclaim_templates as
+      [|physical_claim_template pure_claim_template
+         physical_claim_templates' pure_claim_templates'
+         [Hname Hindex] Hclaim_templates IH];
+    intros physical pure Hrelated; simpl; first done.
+  apply IH.
+  by apply claim_template_maps_related_insert.
+Qed.
+
+Lemma claim_templates_maps_related physical_claim_templates
+    pure_claim_templates :
+  Forall2
+    (λ physical_claim_template pure_claim_template,
+      physical_claim_template.(v1.PersistentVolumeClaim.ObjectMeta').(v1.ObjectMeta.Name') =
+        pure_claim_template.(PersistentVolumeClaimV.ObjectMeta').(ObjectMetaV.Name'))
+    physical_claim_templates pure_claim_templates →
+  claim_template_maps_related
+    (λ physical_claim_template pure_claim_template,
+      ∃ i,
+        physical_claim_templates !! i = Some physical_claim_template ∧
+        pure_claim_templates !! i = Some pure_claim_template)
+    (claim_templates_map_of_list physical_claim_templates)
+    (persistent_volume_claim_templates_by_name pure_claim_templates).
+Proof.
+  intros Hclaim_templates.
+  apply claim_template_maps_related_fold.
+  - by apply Forall2_claim_template_names_with_lookup.
+  - intros name physical_claim_template Hlookup.
+    rewrite lookup_empty in Hlookup. done.
+Qed.
+
+Lemma persistent_volume_claim_template_lookup_acc
+    (claim_templates_phy :
+      gmap go_string v1.PersistentVolumeClaim.t)
+    (claim_templates_list : list v1.PersistentVolumeClaim.t)
+    (claim_templates : list PersistentVolumeClaimV.t)
+    claim_template_name claim_template_phy dq :
+  (∀ name,
+    claim_templates_phy !! name =
+      claim_templates_map_of_list claim_templates_list !! name) →
+  claim_templates_phy !! claim_template_name = Some claim_template_phy →
+  ([∗ list] claim_template_phy;claim_template ∈
+      claim_templates_list;claim_templates,
+      PersistentVolumeClaimV.deepown claim_template_phy claim_template dq) -∗
+  ∃ claim_template,
+    ⌜ persistent_volume_claim_templates_by_name claim_templates !!
+        claim_template_name = Some claim_template ⌝ ∗
+    PersistentVolumeClaimV.deepown
+      claim_template_phy claim_template dq ∗
+    (PersistentVolumeClaimV.deepown
+        claim_template_phy claim_template dq -∗
+     ([∗ list] claim_template_phy;claim_template ∈
+        claim_templates_list;claim_templates,
+        PersistentVolumeClaimV.deepown
+          claim_template_phy claim_template dq)).
+Proof.
+  intros Hmap_eq Hclaim_lookup.
+  iIntros "Hclaim_templates".
+  iDestruct (persistent_volume_claim_deepown_list_names with
+    "Hclaim_templates") as "[%Hnames Hclaim_templates]".
+  assert (Forall2
+      (λ physical_claim_template pure_claim_template,
+        physical_claim_template.(v1.PersistentVolumeClaim.ObjectMeta').(v1.ObjectMeta.Name') =
+          pure_claim_template.(PersistentVolumeClaimV.ObjectMeta').(ObjectMetaV.Name'))
+      claim_templates_list claim_templates) as Hnames_forall2.
+  { apply Forall2_fmap_1.
+    rewrite -list_eq_Forall2.
+    exact Hnames. }
+  pose proof (claim_templates_maps_related _ _ Hnames_forall2)
+    as Hmaps_related.
+  rewrite Hmap_eq in Hclaim_lookup.
+  destruct (Hmaps_related _ _ Hclaim_lookup) as
+    (claim_template & Hclaim_template_lookup & i &
+      Hclaim_phy_lookup & Hclaim_pure_lookup).
+  iDestruct (big_sepL2_lookup_acc _ _ _ i _ _
+    Hclaim_phy_lookup Hclaim_pure_lookup with
+    "Hclaim_templates") as "[Hclaim_template Hclaim_templates]".
+  iExists claim_template.
+  iSplit; first done.
+  iFrame.
+Qed.
 
 (* [createPersistentVolumeClaim] is an idempotent ensure operation.  If the
    claim already exists, Get succeeds and its fragments are preserved.  If its
    key is reserved, the Kubernetes model guarantees that it is absent, so the
    NotFound branch creates it and consumes the reservation. *)
-Lemma wp_createPersistentVolumeClaim γ model_l
+Lemma wp_createPersistentVolumeClaim_without_claim_templates γ model_l
     set_l pod_l claim_template_l
     (set : StatefulSetV.t) (pod : PodV.t)
     (claim_template : PersistentVolumeClaimV.t) (ordinal : nat)
-    dq_set dq_pod dq_claim_template :
+    dq_set dq_pod dq_claim_template_ptr dq_claim_template
+    set_phy claim_template_phy :
   {{{ "#Hpkg" ∷
         is_pkg_init code.controllers.statefulset.pkg_id.statefulset ∗
       "#Hisk" ∷ is_kubernetes γ model_l ∗
       "#Hglobal_l" ∷
         (global_addr apimodel.ModelState) ↦□ model_l ∗
-      "Hset" ∷ StatefulSetV.deepown_l set_l set dq_set ∗
+      "Hset" ∷ statefulset_without_claim_templates_l
+        set_l set dq_set set_phy ∗
       "Hpod" ∷ PodV.deepown_l pod_l pod dq_pod ∗
-      "Hclaim_template" ∷
-        PersistentVolumeClaimV.deepown_l
-          claim_template_l claim_template dq_claim_template ∗
+      "Hclaim_template_ptr" ∷
+        claim_template_l ↦{dq_claim_template_ptr} claim_template_phy ∗
+      "Hclaim_template" ∷ PersistentVolumeClaimV.deepown
+        claim_template_phy claim_template dq_claim_template ∗
       "%Hordinal_bound" ∷
         ⌜ (ordinal ≤ go_int32_max_nat)%nat ⌝ ∗
       "%Hpod_name" ∷
@@ -93,9 +317,16 @@ Lemma wp_createPersistentVolumeClaim γ model_l
             (length pod.(PodV.ObjectMeta').(ObjectMetaV.Name')) ≤
           go_int_max ⌝ ∗
       "Hpvc_state" ∷
-        (persistent_volume_claim_exists γ
-            (new_persistent_volume_claim_key
-              set claim_template ordinal) ∨
+        ((∃ claim,
+            "%Hkey" ∷
+              ⌜ PersistentVolumeClaimV.key claim =
+                new_persistent_volume_claim_key
+                  set claim_template ordinal ⌝ ∗
+            "Hmeta" ∷ own_meta_frag γ
+              (new_persistent_volume_claim_key
+                set claim_template ordinal)
+              claim.(PersistentVolumeClaimV.ObjectMeta').(ObjectMetaV.UID') 1
+              claim.(PersistentVolumeClaimV.ObjectMeta')) ∨
          ("Hreserved" ∷ own_reserved_frag γ
             (new_persistent_volume_claim_key
               set claim_template ordinal) ∗
@@ -114,23 +345,33 @@ Lemma wp_createPersistentVolumeClaim γ model_l
     @! statefulset.createPersistentVolumeClaim
       #set_l #pod_l #claim_template_l
   {{{ RET #interface.nil;
-      "Hset" ∷ StatefulSetV.deepown_l set_l set dq_set ∗
+      "Hset" ∷ statefulset_without_claim_templates_l
+        set_l set dq_set set_phy ∗
       "Hpod" ∷ PodV.deepown_l pod_l pod dq_pod ∗
-      "Hclaim_template" ∷
-        PersistentVolumeClaimV.deepown_l
-          claim_template_l claim_template dq_claim_template ∗
+      "Hclaim_template_ptr" ∷
+        claim_template_l ↦{dq_claim_template_ptr} claim_template_phy ∗
+      "Hclaim_template" ∷ PersistentVolumeClaimV.deepown
+        claim_template_phy claim_template dq_claim_template ∗
       "Hpvc_state" ∷
-        persistent_volume_claim_exists γ
-          (new_persistent_volume_claim_key
-            set claim_template ordinal)
+        (∃ claim,
+          "%Hkey" ∷
+            ⌜ PersistentVolumeClaimV.key claim =
+              new_persistent_volume_claim_key
+                set claim_template ordinal ⌝ ∗
+          "Hmeta" ∷ own_meta_frag γ
+            (new_persistent_volume_claim_key
+              set claim_template ordinal)
+            claim.(PersistentVolumeClaimV.ObjectMeta').(ObjectMetaV.UID') 1
+            claim.(PersistentVolumeClaimV.ObjectMeta'))
   }}}.
 Proof.
   wp_start as "H". iNamed "H".
   wp_auto.
-  wp_apply (wp_newPersistentVolumeClaim
+  wp_apply (wp_newPersistentVolumeClaim_without_claim_templates
     set_l pod_l claim_template_l set pod claim_template ordinal
-    dq_set dq_pod dq_claim_template
-    with "[$Hset $Hpod $Hclaim_template]").
+    dq_set dq_pod dq_claim_template_ptr dq_claim_template
+    set_phy claim_template_phy
+    with "[$Hset $Hpod $Hclaim_template_ptr $Hclaim_template]").
   { iFrame "%". }
   iIntros (claim_l) "H". iNamed "H".
   iPoseProof (PersistentVolumeClaimV.deepown_l_split with "Hclaim") as
@@ -154,8 +395,7 @@ Proof.
       existing_claim.(PersistentVolumeClaimV.ObjectMeta').(ObjectMetaV.UID')
       1
       existing_claim.(PersistentVolumeClaimV.ObjectMeta')
-      existing_claim.(PersistentVolumeClaimV.Spec')
-      with "[$Hmeta $Hspec]").
+      with "[$Hmeta]").
     { iFrame "#".
       iPureIntro.
       unfold new_persistent_volume_claim_key,
@@ -170,7 +410,7 @@ Proof.
       (symmetry; apply bool_decide_false; exact not_found_error_nil).
     wp_auto.
     iApply "HΦ".
-    iFrame "Hset Hpod Hclaim_template".
+    iFrame "Hset Hpod Hclaim_template_ptr Hclaim_template".
     iExists existing_claim.
     iFrame.
     iPureIntro.
@@ -233,12 +473,463 @@ Proof.
     subst uid.
     wp_auto.
     iApply "HΦ".
-    iFrame "Hset Hpod Hclaim_template".
+    iFrame "Hset Hpod Hclaim_template_ptr Hclaim_template".
     iExists created_claim.
     iFrame.
     iPureIntro.
     symmetry.
     exact Hkey_eq'.
+Qed.
+
+Lemma wp_createPersistentVolumeClaim γ model_l
+    set_l pod_l claim_template_l
+    (set : StatefulSetV.t) (pod : PodV.t)
+    (claim_template : PersistentVolumeClaimV.t) (ordinal : nat)
+    dq_set dq_pod dq_claim_template :
+  {{{ "#Hpkg" ∷
+        is_pkg_init code.controllers.statefulset.pkg_id.statefulset ∗
+      "#Hisk" ∷ is_kubernetes γ model_l ∗
+      "#Hglobal_l" ∷
+        (global_addr apimodel.ModelState) ↦□ model_l ∗
+      "Hset" ∷ StatefulSetV.deepown_l set_l set dq_set ∗
+      "Hpod" ∷ PodV.deepown_l pod_l pod dq_pod ∗
+      "Hclaim_template" ∷
+        PersistentVolumeClaimV.deepown_l
+          claim_template_l claim_template dq_claim_template ∗
+      "%Hordinal_bound" ∷
+        ⌜ (ordinal ≤ go_int32_max_nat)%nat ⌝ ∗
+      "%Hpod_name" ∷
+        ⌜ pod.(PodV.ObjectMeta').(ObjectMetaV.Name') =
+            desired_pod_name
+              set.(StatefulSetV.ObjectMeta').(ObjectMetaV.Name')
+              ordinal ⌝ ∗
+      "%Hpod_name_len" ∷
+        ⌜ Z.of_nat
+            (length pod.(PodV.ObjectMeta').(ObjectMetaV.Name')) ≤
+          go_int_max ⌝ ∗
+      "Hpvc_state" ∷
+        ((∃ claim,
+            "%Hkey" ∷
+              ⌜ PersistentVolumeClaimV.key claim =
+                new_persistent_volume_claim_key
+                  set claim_template ordinal ⌝ ∗
+            "Hmeta" ∷ own_meta_frag γ
+              (new_persistent_volume_claim_key
+                set claim_template ordinal)
+              claim.(PersistentVolumeClaimV.ObjectMeta').(ObjectMetaV.UID') 1
+              claim.(PersistentVolumeClaimV.ObjectMeta')) ∨
+         ("Hreserved" ∷ own_reserved_frag γ
+            (new_persistent_volume_claim_key
+              set claim_template ordinal) ∗
+          "%Hvalid_create" ∷
+            ⌜ PersistentVolumeClaimV.valid_named_create
+                set.(StatefulSetV.ObjectMeta').(ObjectMetaV.Namespace')
+                (new_persistent_volume_claim
+                  set claim_template ordinal) ⌝ ∗
+          "%Hnamespace_nonempty" ∷
+            ⌜ set.(StatefulSetV.ObjectMeta').(ObjectMetaV.Namespace') ≠
+                ""%go ⌝ ∗
+          "%Hnamespace_valid" ∷
+            ⌜ valid_namespace
+                set.(StatefulSetV.ObjectMeta').(ObjectMetaV.Namespace') ⌝))
+  }}}
+    @! statefulset.createPersistentVolumeClaim
+      #set_l #pod_l #claim_template_l
+  {{{ RET #interface.nil;
+      "Hset" ∷ StatefulSetV.deepown_l set_l set dq_set ∗
+      "Hpod" ∷ PodV.deepown_l pod_l pod dq_pod ∗
+      "Hclaim_template" ∷
+        PersistentVolumeClaimV.deepown_l
+          claim_template_l claim_template dq_claim_template ∗
+      "Hpvc_state" ∷
+        (∃ claim,
+          "%Hkey" ∷
+            ⌜ PersistentVolumeClaimV.key claim =
+              new_persistent_volume_claim_key
+                set claim_template ordinal ⌝ ∗
+          "Hmeta" ∷ own_meta_frag γ
+            (new_persistent_volume_claim_key
+              set claim_template ordinal)
+            claim.(PersistentVolumeClaimV.ObjectMeta').(ObjectMetaV.UID') 1
+            claim.(PersistentVolumeClaimV.ObjectMeta'))
+  }}}.
+Proof.
+  iIntros (Φ) "H HΦ". iNamed "H".
+  iDestruct "Hset" as (set_phy) "[Hset_ptr Hset]".
+  iNamed "Hset".
+  iNamed "Hdeepown_spec".
+  iDestruct "Hdeepown_volumeclaimtemplates" as
+    (claim_templates_list) "Hdeepown_volumeclaimtemplates".
+  iDestruct "Hclaim_template" as (claim_template_phy)
+    "[Hclaim_template_ptr Hclaim_template]".
+  iAssert (statefulset_without_claim_templates_l
+      set_l set dq_set set_phy)
+    with "[Hset_ptr Hdeepown_objectmeta
+      Hdeepown_replicas_some Hdeepown_selector_some
+      Hdeepown_template Hdeepown_status]" as "Hset".
+  { rewrite /statefulset_without_claim_templates_l.
+    iFrame. iFrame "%". }
+  wp_apply (wp_createPersistentVolumeClaim_without_claim_templates
+    γ model_l set_l pod_l claim_template_l set pod claim_template ordinal
+    dq_set dq_pod dq_claim_template dq_claim_template
+    set_phy claim_template_phy
+    with "[$Hset $Hpod $Hclaim_template_ptr
+      $Hclaim_template $Hpvc_state]").
+  { iFrame "# %". }
+  iIntros "H". iNamed "H".
+  iAssert (PersistentVolumeClaimV.deepown_l
+      claim_template_l claim_template dq_claim_template)
+    with "[Hclaim_template_ptr Hclaim_template]"
+    as "Hclaim_template_l".
+  { iExists claim_template_phy. iFrame. }
+  iNamed "Hset".
+  iAssert (StatefulSetV.deepown_l set_l set dq_set)
+    with "[Hset_ptr Hdeepown_objectmeta
+      Hset_spec_Hdeepown_replicas_some
+      Hset_spec_Hdeepown_selector_some
+      Hset_spec_Hdeepown_template Hdeepown_volumeclaimtemplates
+      Hdeepown_status]" as "Hset".
+  { iExists set_phy.
+    rewrite /StatefulSetV.deepown /StatefulSetSpecV.deepown.
+    iFrame.
+    iFrame "%". }
+  iApply "HΦ".
+  iFrame "Hset Hpod Hclaim_template_l Hpvc_state".
+Qed.
+
+(* [volumeClaimTemplatesByName] indexes templates by name before this function
+   iterates over them.  The specification consequently tracks one PVC state per
+   distinct template name, matching both the controller implementation and the
+   top-level [desired_pvc_keys] progress invariant. *)
+Lemma wp_createPersistentVolumeClaims γ model_l set_l pod_l
+    (set : StatefulSetV.t) (pod : PodV.t) (ordinal : nat)
+    dq_set dq_pod :
+  {{{ "#Hpkg" ∷
+        is_pkg_init code.controllers.statefulset.pkg_id.statefulset ∗
+      "#Hisk" ∷ is_kubernetes γ model_l ∗
+      "#Hglobal_l" ∷
+        (global_addr apimodel.ModelState) ↦□ model_l ∗
+      "Hset" ∷ StatefulSetV.deepown_l set_l set dq_set ∗
+      "Hpod" ∷ PodV.deepown_l pod_l pod dq_pod ∗
+      "%Hordinal_bound" ∷
+        ⌜ (ordinal ≤ go_int32_max_nat)%nat ⌝ ∗
+      "%Hpod_name" ∷
+        ⌜ pod.(PodV.ObjectMeta').(ObjectMetaV.Name') =
+            desired_pod_name
+              set.(StatefulSetV.ObjectMeta').(ObjectMetaV.Name')
+              ordinal ⌝ ∗
+      "%Hpod_name_len" ∷
+        ⌜ Z.of_nat
+            (length pod.(PodV.ObjectMeta').(ObjectMetaV.Name')) ≤
+          go_int_max ⌝ ∗
+      "%Hnamespace_nonempty" ∷
+        ⌜ set.(StatefulSetV.ObjectMeta').(ObjectMetaV.Namespace') ≠
+            ""%go ⌝ ∗
+      "%Hnamespace_valid" ∷
+        ⌜ valid_namespace
+            set.(StatefulSetV.ObjectMeta').(ObjectMetaV.Namespace') ⌝ ∗
+      "Hpvc_states" ∷
+        ([∗ map] claim_template_name↦claim_template ∈
+          persistent_volume_claim_templates_by_name
+            set.(StatefulSetV.Spec').(StatefulSetSpecV.VolumeClaimTemplates'),
+          (∃ claim,
+            "%Hkey" ∷
+              ⌜ PersistentVolumeClaimV.key claim =
+                desired_pvc_key set claim_template_name ordinal ⌝ ∗
+            "Hmeta" ∷ own_meta_frag γ
+              (desired_pvc_key set claim_template_name ordinal)
+              claim.(PersistentVolumeClaimV.ObjectMeta').(ObjectMetaV.UID') 1
+              claim.(PersistentVolumeClaimV.ObjectMeta')) ∨
+          (own_reserved_frag γ
+              (desired_pvc_key set claim_template_name ordinal) ∗
+           ⌜ PersistentVolumeClaimV.valid_named_create
+                set.(StatefulSetV.ObjectMeta').(ObjectMetaV.Namespace')
+                (new_persistent_volume_claim
+                  set claim_template ordinal) ⌝))
+  }}}
+    @! statefulset.createPersistentVolumeClaims #set_l #pod_l
+  {{{ RET #interface.nil;
+      "Hset" ∷ StatefulSetV.deepown_l set_l set dq_set ∗
+      "Hpod" ∷ PodV.deepown_l pod_l pod dq_pod ∗
+      "Hpvc_states" ∷
+        ([∗ set] claim_template_name ∈
+          list_to_set (pvc_claim_template_names set),
+          ∃ claim,
+            "%Hkey" ∷
+              ⌜ PersistentVolumeClaimV.key claim =
+                desired_pvc_key set claim_template_name ordinal ⌝ ∗
+            "Hmeta" ∷ own_meta_frag γ
+              (desired_pvc_key set claim_template_name ordinal)
+              claim.(PersistentVolumeClaimV.ObjectMeta').(ObjectMetaV.UID') 1
+              claim.(PersistentVolumeClaimV.ObjectMeta'))
+  }}}.
+Proof.
+  wp_start as "H". iNamed "H".
+  wp_auto.
+  wp_apply (wp_volumeClaimTemplatesByName set_l set dq_set with "Hset").
+  iIntros (set_phy claim_templates_map claim_templates_list
+    claim_templates_phy) "H".
+  iDestruct "H" as "[Hset_ptr H]".
+  iDestruct "H" as
+    "(%Hdeepown_typemeta & Hdeepown_objectmeta &
+      %Hdeepown_replicas_none & Hdeepown_replicas_some &
+      %Hdeepown_selector_none & Hdeepown_selector_some &
+      Hdeepown_template & Hdeepown_volumeclaimtemplates &
+      %Hclaim_templates_map_values & %Hclaim_templates_list_names &
+      %Hclaim_templates_map_dom & %Hclaim_templates_map_eq &
+      %Hdeepown_servicename &
+      Hdeepown_status & Hclaim_templates_map)".
+  iEval (rewrite /deepown_list) in "Hdeepown_volumeclaimtemplates".
+  iDestruct "Hdeepown_volumeclaimtemplates" as
+    "[Hclaim_templates_slice Hclaim_templates_deepown]".
+  iAssert (statefulset_without_claim_templates_l
+      set_l set dq_set set_phy)
+    with "[Hset_ptr Hdeepown_objectmeta
+      Hdeepown_replicas_some Hdeepown_selector_some
+      Hdeepown_template Hdeepown_status]" as "Hset".
+  { rewrite /statefulset_without_claim_templates_l.
+    iFrame. iFrame "%". }
+
+  set claim_templates :=
+    set.(StatefulSetV.Spec').(StatefulSetSpecV.VolumeClaimTemplates').
+  set claim_templates_pure :=
+    persistent_volume_claim_templates_by_name claim_templates.
+  set pvc_ready := (λ claim_template_name claim_template,
+    (∃ claim,
+      "%Hkey" ∷
+        ⌜ PersistentVolumeClaimV.key claim =
+          desired_pvc_key set claim_template_name ordinal ⌝ ∗
+      "Hmeta" ∷ own_meta_frag γ
+        (desired_pvc_key set claim_template_name ordinal)
+        claim.(PersistentVolumeClaimV.ObjectMeta').(ObjectMetaV.UID') 1
+        claim.(PersistentVolumeClaimV.ObjectMeta')) ∨
+    (own_reserved_frag γ
+        (desired_pvc_key set claim_template_name ordinal) ∗
+     ⌜ PersistentVolumeClaimV.valid_named_create
+          set.(StatefulSetV.ObjectMeta').(ObjectMetaV.Namespace')
+          (new_persistent_volume_claim
+            set claim_template ordinal) ⌝))%I.
+  set pvc_done := (λ claim_template_name,
+    ∃ claim,
+      "%Hkey" ∷
+        ⌜ PersistentVolumeClaimV.key claim =
+          desired_pvc_key set claim_template_name ordinal ⌝ ∗
+      "Hmeta" ∷ own_meta_frag γ
+        (desired_pvc_key set claim_template_name ordinal)
+        claim.(PersistentVolumeClaimV.ObjectMeta').(ObjectMetaV.UID') 1
+        claim.(PersistentVolumeClaimV.ObjectMeta'))%I.
+  assert (Hclaim_templates_pure_dom :
+      dom claim_templates_pure = dom claim_templates_phy).
+  { unfold_leibniz.
+    apply set_equiv. intros claim_template_name.
+    rewrite Hclaim_templates_map_dom /claim_templates_pure
+      persistent_volume_claim_templates_by_name_dom.
+    done. }
+  assert (Hclaim_templates_pure_size :
+      size claim_templates_pure = size claim_templates_phy).
+  { pose proof (f_equal size Hclaim_templates_pure_dom) as Hsize.
+    rewrite !size_dom in Hsize.
+    exact Hsize. }
+  iAssert (([∗ map] name↦claim_template ∈ claim_templates_pure,
+      pvc_ready name claim_template))%I
+    with "[Hpvc_states]" as "Hpvc_todo".
+  { rewrite /claim_templates_pure.
+    iExact "Hpvc_states". }
+  wp_auto.
+  set P := (λ (keys : list go_string) (z : Z),
+    ∃ (last_claim_template : v1.PersistentVolumeClaim.t),
+      "set" ∷ set_ptr ↦ set_l ∗
+      "pod" ∷ pod_ptr ↦ pod_l ∗
+      "claimTemplate" ∷ claimTemplate_ptr ↦ last_claim_template ∗
+      "Hset" ∷ statefulset_without_claim_templates_l
+        set_l set dq_set set_phy ∗
+      "Hpod" ∷ PodV.deepown_l pod_l pod dq_pod ∗
+      "Hclaim_templates_slice" ∷
+        set_phy.(v1.StatefulSet.Spec').(v1.StatefulSetSpec.VolumeClaimTemplates')
+          ↦* claim_templates_list ∗
+      "Hclaim_templates_deepown" ∷
+        ([∗ list] claim_template_phy;claim_template ∈
+          claim_templates_list;claim_templates,
+          PersistentVolumeClaimV.deepown
+            claim_template_phy claim_template dq_set) ∗
+      "Hpvc_done" ∷
+        ([∗ map] name↦claim_template ∈
+          map_prefix keys z claim_templates_pure,
+          pvc_done name) ∗
+      "Hpvc_todo" ∷
+        ([∗ map] name↦claim_template ∈
+          claim_templates_pure ∖
+            map_prefix keys z claim_templates_pure,
+          pvc_ready name claim_template))%I.
+  wp_apply (wp_map_for_range_return (key_type:=go.string) P
+    with "Hclaim_templates_map").
+  iIntros (keys) "%Hkeys".
+  destruct Hkeys as (Hkeys_dom & Hkeys_len & Hkeys_nodup).
+  iSplitL "set pod claimTemplate Hset Hpod
+      Hclaim_templates_slice Hclaim_templates_deepown Hpvc_todo".
+  { iExists (zero_val v1.PersistentVolumeClaim.t).
+    rewrite map_prefix_empty map_difference_empty big_sepM_empty.
+    iFrame. }
+  iSplitL "".
+  { iModIntro.
+    iIntros (z claim_template_name claim_template_phy)
+      "%Hiter HP".
+    destruct Hiter as (Hz_bounds & Hkey_lookup & Hclaim_lookup).
+    destruct Hz_bounds as (Hz_nonneg & Hz_upper).
+    iDestruct "HP" as (last_claim_template) "HP".
+    iNamed "HP".
+    assert (Hclaim_template_name_not_processed :
+        claim_template_name ∉ take (Z.to_nat z) keys).
+    { intros Hin.
+      rewrite elem_of_take in Hin.
+      destruct Hin as (i & Hi_lookup & Hi_lt).
+      pose proof (NoDup_lookup keys i (Z.to_nat z)
+        claim_template_name Hkeys_nodup Hi_lookup Hkey_lookup).
+      lia. }
+    assert (Hprefix_lookup :
+        map_prefix keys z claim_templates_pure !!
+          claim_template_name = None).
+    { rewrite /map_prefix map_lookup_filter_None.
+      right.
+      intros claim_template Hlookup Hin.
+      apply Hclaim_template_name_not_processed.
+      rewrite elem_of_list_to_set in Hin.
+      exact Hin. }
+    iDestruct
+      (persistent_volume_claim_template_lookup_acc
+        claim_templates_phy claim_templates_list claim_templates
+        claim_template_name claim_template_phy dq_set
+        Hclaim_templates_map_eq Hclaim_lookup
+        with "Hclaim_templates_deepown")
+      as (claim_template)
+        "(%Hclaim_template_lookup & Hclaim_template &
+          Hclaim_templates_restore)".
+    pose proof (Hclaim_templates_map_values _ _ Hclaim_lookup) as
+      [_ Hclaim_template_phy_name].
+    iDestruct (persistent_volume_claim_deepown_name with
+      "Hclaim_template") as
+      "[%Hclaim_template_deepown_name Hclaim_template]".
+    assert (Hclaim_template_name :
+        claim_template.(PersistentVolumeClaimV.ObjectMeta').(ObjectMetaV.Name') =
+          claim_template_name) by congruence.
+    assert (Htodo_lookup :
+        (claim_templates_pure ∖
+          map_prefix keys z claim_templates_pure) !!
+          claim_template_name = Some claim_template).
+    { rewrite lookup_difference_Some.
+      split; done. }
+    iDestruct (big_sepM_delete _ _ _ _ Htodo_lookup with
+      "Hpvc_todo") as "[Hpvc_state Hpvc_todo]".
+    wp_auto.
+    iAssert
+      ((∃ claim,
+          "%Hkey" ∷
+            ⌜ PersistentVolumeClaimV.key claim =
+              new_persistent_volume_claim_key
+                set claim_template ordinal ⌝ ∗
+          "Hmeta" ∷ own_meta_frag γ
+            (new_persistent_volume_claim_key
+              set claim_template ordinal)
+            claim.(PersistentVolumeClaimV.ObjectMeta').(ObjectMetaV.UID') 1
+            claim.(PersistentVolumeClaimV.ObjectMeta')) ∨
+       (own_reserved_frag γ
+          (new_persistent_volume_claim_key
+            set claim_template ordinal) ∗
+        ⌜ PersistentVolumeClaimV.valid_named_create
+            set.(StatefulSetV.ObjectMeta').(ObjectMetaV.Namespace')
+            (new_persistent_volume_claim
+              set claim_template ordinal) ⌝ ∗
+        ⌜ set.(StatefulSetV.ObjectMeta').(ObjectMetaV.Namespace') ≠
+            ""%go ⌝ ∗
+        ⌜ valid_namespace
+            set.(StatefulSetV.ObjectMeta').(ObjectMetaV.Namespace') ⌝))%I
+      with "[Hpvc_state]" as "Hpvc_state".
+    { rewrite new_persistent_volume_claim_key_eq
+        Hclaim_template_name /pvc_ready.
+      iDestruct "Hpvc_state" as "[Hpvc_state | Hpvc_state]".
+      - iLeft. iExact "Hpvc_state".
+      - iDestruct "Hpvc_state" as "[Hreserved %Hvalid_create]".
+        iRight.
+        iFrame "Hreserved".
+        iFrame "%". }
+    wp_apply
+      (wp_createPersistentVolumeClaim_without_claim_templates
+        γ model_l set_l pod_l claimTemplate_ptr set pod
+        claim_template ordinal dq_set dq_pod 1 dq_set set_phy
+        claim_template_phy
+        with "[$Hset $Hpod $claimTemplate
+          $Hclaim_template $Hpvc_state]").
+    { iFrame "# %". }
+    iIntros "H". iNamed "H".
+    iEval (rewrite new_persistent_volume_claim_key_eq
+      Hclaim_template_name) in "Hpvc_state".
+    iSpecialize ("Hclaim_templates_restore" with "Hclaim_template").
+    iRename "Hclaim_templates_restore" into
+      "Hclaim_templates_deepown".
+    wp_auto.
+    assert (Hprefix_next :
+        map_prefix keys (z + 1) claim_templates_pure =
+          <[claim_template_name:=claim_template]>
+            (map_prefix keys z claim_templates_pure)).
+    { apply map_prefix_insert; done. }
+    iRight. iSplit; first done.
+    iExists claim_template_phy.
+    iFrame "set pod Hset Hpod Hclaim_template_ptr
+      Hclaim_templates_slice Hclaim_templates_deepown".
+    rewrite Hprefix_next.
+    iSplitL "Hpvc_done Hpvc_state".
+    - rewrite (big_sepM_insert
+        (λ name _, pvc_done name)%I
+        (map_prefix keys z claim_templates_pure)
+        claim_template_name claim_template Hprefix_lookup).
+      iFrame.
+    - rewrite <-(delete_difference claim_templates_pure
+        (map_prefix keys z claim_templates_pure)
+        claim_template_name claim_template).
+      iExact "Hpvc_todo".
+  }
+  iIntros "Hclaim_templates_map HP".
+  iDestruct "HP" as (last_claim_template) "HP".
+  iNamed "HP".
+  assert (Hprefix_all :
+      map_prefix keys (Z.of_nat (size claim_templates_pure))
+        claim_templates_pure = claim_templates_pure).
+  { apply map_prefix_all.
+    - rewrite Hclaim_templates_pure_dom. exact Hkeys_dom.
+    - rewrite Hclaim_templates_pure_size. exact Hkeys_len. }
+  rewrite Hclaim_templates_pure_size in Hprefix_all.
+  iEval (rewrite Hprefix_all) in "Hpvc_done".
+  iEval (rewrite Hprefix_all map_difference_diag big_sepM_empty)
+    in "Hpvc_todo".
+  iClear "Hpvc_todo".
+  iAssert (([∗ set] claim_template_name ∈ dom claim_templates_pure,
+      pvc_done claim_template_name))%I
+    with "[Hpvc_done]" as "Hpvc_states".
+  { rewrite -big_sepM_dom.
+    iExact "Hpvc_done". }
+  iNamed "Hset".
+  iAssert (StatefulSetV.deepown_l set_l set dq_set)
+    with "[Hset_ptr Hdeepown_objectmeta
+      Hset_spec_Hdeepown_replicas_some
+      Hset_spec_Hdeepown_selector_some
+      Hset_spec_Hdeepown_template Hclaim_templates_slice
+      Hclaim_templates_deepown Hdeepown_status]" as "Hset".
+  { iExists set_phy.
+    rewrite /StatefulSetV.deepown /StatefulSetSpecV.deepown.
+    iFrame "Hset_ptr Hdeepown_objectmeta
+      Hset_spec_Hdeepown_replicas_some
+      Hset_spec_Hdeepown_selector_some
+      Hset_spec_Hdeepown_template Hdeepown_status".
+    iFrame "%".
+    iExists claim_templates_list.
+    rewrite /deepown_list.
+    iFrame. }
+  wp_auto.
+  iApply "HΦ".
+  rewrite /pvc_done /claim_templates_pure
+    persistent_volume_claim_templates_by_name_dom
+    /claim_templates /pvc_claim_template_names.
+  iFrame.
 Qed.
 
 End proof.
