src/proof/kubernetes_model/get.v
@@ -384,8 +384,7 @@ Proof.
   iApply ("HΦ" with "Hpost").
 Qed.
 
-Lemma wp_State__PersistentVolumeClaimMutGet γ l key namespace name uid dq
-    kmeta kspec :
+Lemma wp_State__PersistentVolumeClaimMutGet γ l key namespace name uid dq kmeta :
   {{{ is_pkg_init apimodel ∗
       "#Hisk" ∷ is_kubernetes γ l ∗
       "%Hkey_def" ∷ ⌜ key = {|
@@ -393,12 +392,9 @@ Lemma wp_State__PersistentVolumeClaimMutGet γ l key namespace name uid dq
         KKey.Namespace' := namespace;
         KKey.Name' := name
       |} ⌝ ∗
-      "Hown_meta_frag" ∷ own_meta_frag γ key uid dq kmeta ∗
-      "Hown_spec_frag" ∷ own_spec_frag γ key uid dq
-        (ObjectSpecV.PersistentVolumeClaimSpec kspec)
+      "Hown_meta_frag" ∷ own_meta_frag γ key uid dq kmeta
   }}}
-    l @! (go.PointerType apimodel.State) @!
-      "PersistentVolumeClaimMutGet" #namespace #name
+    l @! (go.PointerType apimodel.State) @! "PersistentVolumeClaimMutGet" #namespace #name
   {{{ pvc_l pvc, RET (#pvc_l, #interface.nil);
       "%Hvalid'" ∷
         ⌜ KObjectV.valid (KObjectV.PersistentVolumeClaim pvc) ⌝ ∗
@@ -406,33 +402,40 @@ Lemma wp_State__PersistentVolumeClaimMutGet γ l key namespace name uid dq
       "%Hmeta_eq" ∷
         ⌜ ObjectMetaV.equiv_except_resource_version
             pvc.(PersistentVolumeClaimV.ObjectMeta') kmeta ⌝ ∗
-      "%Hspec_eq" ∷ ⌜ kspec = pvc.(PersistentVolumeClaimV.Spec') ⌝ ∗
       "Hdeepown_l" ∷ PersistentVolumeClaimV.deepown_l pvc_l pvc 1 ∗
-      "Hown_meta_frag" ∷ own_meta_frag γ key uid dq kmeta ∗
-      "Hown_spec_frag" ∷ own_spec_frag γ key uid dq
-        (ObjectSpecV.PersistentVolumeClaimSpec kspec)
+      "Hown_meta_frag" ∷ own_meta_frag γ key uid dq kmeta
   }}}.
 Proof.
   iIntros (Φ) "(#Hinit & H) HΦ". iNamed "H". subst key.
   wp_method_call.
   rewrite /apimodel.State__PersistentVolumeClaimMutGetⁱᵐᵖˡ.
   wp_call. wp_auto.
+  iAssert (is_pkg_init apimodel ∗
+      is_kubernetes γ l ∗
+      own_meta_frag γ
+        {| KKey.Kind' := "PersistentVolumeClaim"%go;
+           KKey.Namespace' := namespace;
+           KKey.Name' := name |}
+        uid dq kmeta ∗ True ∗ True)%I
+    with "[$Hinit $Hisk $Hown_meta_frag]" as "Hget".
+  { iFrame. done. }
   wp_apply (wp_State__get_some γ l
     {| KKey.Kind' := "PersistentVolumeClaim"%go;
        KKey.Namespace' := namespace;
        KKey.Name' := name |}
     uid dq kmeta
-    (Some (ObjectSpecV.PersistentVolumeClaimSpec kspec)) None
-    with "[$Hinit $Hisk $Hown_meta_frag $Hown_spec_frag]").
+    (None : option ObjectSpecV.t) (None : option ObjectStatusV.t)
+    with "Hget").
   iIntros (i kobj) "Hpost". iNamed "Hpost".
-  iDestruct "Hpost" as "((Hown_spec_frag & %Hspec_eq) & _)".
+  iDestruct "Hpost" as "(_ & _)".
   destruct kobj as [pod|rs|pvc|sts];
-    try solve [simpl in Hspec_eq; done].
-  simpl in Hvalid', Hkey_eq, Hmeta_eq, Hspec_eq.
-  assert (Hspec_eq' : kspec = pvc.(PersistentVolumeClaimV.Spec'))
-    by congruence.
-  clear Hspec_eq.
-  rename Hspec_eq' into Hspec_eq.
+    try solve [
+      exfalso;
+      apply (f_equal KKey.Kind') in Hkey_eq;
+      simpl in Hkey_eq;
+      discriminate
+    ].
+  simpl in Hvalid', Hkey_eq, Hmeta_eq.
   iDestruct "Hdeepown_i" as (pvc_l) "[%Hi Hdeepown_l]".
   wp_auto.
   unfold KObjectV.valid_interface in Hi. rewrite Hi.
@@ -454,8 +457,7 @@ Proof.
   iApply "HΦ". iFrame. iPureIntro. split_and!; done.
 Qed.
 
-Lemma wp_State__PersistentVolumeClaimGet γ l key namespace name uid dq
-    kmeta kspec :
+Lemma wp_State__PersistentVolumeClaimGet γ l key namespace name uid dq kmeta :
   {{{ is_pkg_init apimodel ∗
       "#Hisk" ∷ is_kubernetes γ l ∗
       "%Hkey_def" ∷ ⌜ key = {|
@@ -463,12 +465,9 @@ Lemma wp_State__PersistentVolumeClaimGet γ l key namespace name uid dq
         KKey.Namespace' := namespace;
         KKey.Name' := name
       |} ⌝ ∗
-      "Hown_meta_frag" ∷ own_meta_frag γ key uid dq kmeta ∗
-      "Hown_spec_frag" ∷ own_spec_frag γ key uid dq
-        (ObjectSpecV.PersistentVolumeClaimSpec kspec)
+      "Hown_meta_frag" ∷ own_meta_frag γ key uid dq kmeta
   }}}
-    l @! (go.PointerType apimodel.State) @!
-      "PersistentVolumeClaimGet" #namespace #name
+    l @! (go.PointerType apimodel.State) @! "PersistentVolumeClaimGet" #namespace #name
   {{{ pvc_l pvc, RET (#pvc_l, #interface.nil);
       "%Hvalid'" ∷
         ⌜ KObjectV.valid (KObjectV.PersistentVolumeClaim pvc) ⌝ ∗
@@ -476,11 +475,8 @@ Lemma wp_State__PersistentVolumeClaimGet γ l key namespace name uid dq
       "%Hmeta_eq" ∷
         ⌜ ObjectMetaV.equiv_except_resource_version
             pvc.(PersistentVolumeClaimV.ObjectMeta') kmeta ⌝ ∗
-      "%Hspec_eq" ∷ ⌜ kspec = pvc.(PersistentVolumeClaimV.Spec') ⌝ ∗
       "Hdeepown_l" ∷ PersistentVolumeClaimV.deepown_l pvc_l pvc 1 ∗
-      "Hown_meta_frag" ∷ own_meta_frag γ key uid dq kmeta ∗
-      "Hown_spec_frag" ∷ own_spec_frag γ key uid dq
-        (ObjectSpecV.PersistentVolumeClaimSpec kspec)
+      "Hown_meta_frag" ∷ own_meta_frag γ key uid dq kmeta
   }}}.
 Proof.
   iIntros (Φ) "(#Hinit & H) HΦ". iNamed "H".
@@ -488,33 +484,12 @@ Proof.
   rewrite /apimodel.State__PersistentVolumeClaimGetⁱᵐᵖˡ.
   wp_call. wp_auto.
   wp_apply (wp_State__PersistentVolumeClaimMutGet
-    γ l key namespace name uid dq kmeta kspec
-    with "[$Hinit $Hisk $Hown_meta_frag $Hown_spec_frag]").
+    γ l key namespace name uid dq kmeta
+    with "[$Hinit $Hisk $Hown_meta_frag]").
   { iPureIntro. done. }
   iIntros (pvc_l pvc) "Hpost".
   wp_auto.
   iApply ("HΦ" with "Hpost").
 Qed.
-
-(* The public typed Get wrapper maps the absent result from [State.get] to a
-   Kubernetes StatusError classified as NotFound.  Its physical construction
-   remains behind the same opaque API-errors boundary as [wp_State__get]. *)
-Lemma wp_State__PersistentVolumeClaimGet_reserved γ l key namespace name :
-  {{{ is_pkg_init apimodel ∗
-      "#Hisk" ∷ is_kubernetes γ l ∗
-      "%Hkey_def" ∷ ⌜ key = {|
-        KKey.Kind' := "PersistentVolumeClaim"%go;
-        KKey.Namespace' := namespace;
-        KKey.Name' := name
-      |} ⌝ ∗
-      "Hown_reserved_frag" ∷ own_reserved_frag γ key
-  }}}
-    l @! (go.PointerType apimodel.State) @!
-      "PersistentVolumeClaimGet" #namespace #name
-  {{{ err, RET (#null, #err);
-      "%Hnot_found" ∷ ⌜ not_found_error err ⌝ ∗
-      "Hown_reserved_frag" ∷ own_reserved_frag γ key
-  }}}.
-Proof. Admitted.
 
 End proof.
